wip on converting to coqutil word and map

src/MachineWidth32.v
@@ -1,6 +1,10 @@
+Require Import Coq.ZArith.ZArith.
 Require Import riscv.Utility.
 Require Import riscv.MachineWidth_XLEN.
+Local Open Scope Z_scope.
 
-Instance MachineWidth32: MachineWidth (word 32) := MachineWidth_XLEN 32 _.
-  cbv. discriminate.
-Defined.
+Lemma bound832: 8 <= 32. cbv. discriminate. Qed.
+
+Definition word32: Type := word_sz 32 bound832.
+
+Instance MachineWidth32: MachineWidth word32 := MachineWidth_XLEN 32 bound832.
